characteristic/examples/patchProgScript.sml
@@ -1,0 +1,126 @@
+open preamble ml_translatorLib ml_progLib
+     cfTacticsLib basisFunctionsLib
+     rofsFFITheory mlfileioProgTheory ioProgTheory
+     charsetTheory diffTheory mlstringTheory;
+
+val _ = new_theory "patchProg";
+
+val _ = translation_extends"ioProg";
+
+fun def_of_const tm = let
+  val res = dest_thy_const tm handle HOL_ERR _ =>
+              failwith ("Unable to translate: " ^ term_to_string tm)
+  val name = (#Name res)
+  fun def_from_thy thy name =
+    DB.fetch thy (name ^ "_def") handle HOL_ERR _ =>
+    DB.fetch thy (name ^ "_DEF") handle HOL_ERR _ =>
+    DB.fetch thy (name ^ "_thm") handle HOL_ERR _ =>
+    DB.fetch thy name
+  val def = def_from_thy (#Thy res) name handle HOL_ERR _ =>
+            failwith ("Unable to find definition of " ^ name)
+  in def end
+
+val _ = find_def_for_const := def_of_const;
+
+(* Circumvents a problem where the translator generates unprovable side conditions
+   for higher-order functions *)
+val unhex_all_def = Define `(unhex_all [] = []) /\ (unhex_all (a::b) = UNHEX a::unhex_all b)`
+
+val unhex_map = Q.prove(`!s. unhex_all s = MAP UNHEX s`, Induct >> fs[unhex_all_def])
+
+val s2n_UNHEX_def = Define `s2n_UNHEX b s = l2n b (unhex_all (REVERSE s))`
+
+val num_from_dec_string_thm = Q.store_thm("num_from_dec_string_thm",
+  `!s. toNum s = s2n_UNHEX 10 s`,
+  rw[ASCIInumbersTheory.num_from_dec_string_def,s2n_UNHEX_def,ASCIInumbersTheory.s2n_def,
+     unhex_map]);
+
+val _ = translate num_from_dec_string_thm;
+
+val l2n_side_IMP = Q.prove(`∀n l. n <> 0 ==> l2n_side n l = T`,
+  strip_tac >> Induct >> rw[Once(fetch "-" "l2n_side_def")]);
+
+val unhex_side = Q.prove(`!c. unhex_side c <=> isHexDigit c`,
+  Cases >> fs[isHexDigit_def] >> PURE_ONCE_REWRITE_TAC[fetch "-" "unhex_side_def"]
+        >> PURE_REWRITE_TAC[AC DISJ_ASSOC DISJ_COMM]
+        >> PURE_REWRITE_TAC [GSYM DISJ_ASSOC,AND_CLAUSES]
+        >> PURE_ONCE_REWRITE_TAC[EQ_IMP_THM]
+        >> rpt strip_tac >> rfs[CHR_11]) |> update_precondition
+
+val unhex_all_side = Q.prove(`!s. unhex_all_side s <=> EVERY isHexDigit s`,
+  Induct >> PURE_ONCE_REWRITE_TAC[fetch "-" "unhex_all_side_def"]>> fs[unhex_side])
+  |> update_precondition;
+                        
+val s2n_unhex_side_IMP = Q.prove(`∀n s. n <> 0 ==> s2n_unhex_side n s = EVERY isHexDigit s`,
+  rpt strip_tac
+  >> rw[Once(fetch "-" "s2n_unhex_side_def"),l2n_side_IMP,unhex_all_side,EVERY_REVERSE]);
+
+val num_from_dec_string_side = Q.prove(`
+  ∀s. num_from_dec_string_side s = EVERY isHexDigit s`,
+  fs[fetch "-" "num_from_dec_string_side_def",s2n_unhex_side_IMP]) |> update_precondition;
+
+val _ = translate parse_patch_header_def;
+
+fetch "-" "fromstring_side_def"
+
+val tokens_less_eq = Q.prove(`!s f. EVERY (\x. strlen x <= strlen s) (tokens f s)`,
+  Induct >> Ho_Rewrite.PURE_ONCE_REWRITE_TAC[SWAP_FORALL_THM]
+  >> PURE_ONCE_REWRITE_TAC[TOKENS_eq_tokens_sym]
+  >> recInduct TOKENS_ind >> rpt strip_tac
+  >> fs[TOKENS_def] >> pairarg_tac >> reverse(Cases_on `l`) >> rw[]
+  >- (drule SPLITP_JOIN >> fs[implode_def,strlen_def])
+  >> fs[SPLITP_NIL_FST,SPLITP] >> every_case_tac >> fs[]
+  >- (`!x. (λx. strlen x <= STRLEN r) x ==> (λx. strlen x <= SUC (STRLEN t)) x`
+       by(rpt strip_tac >> PURE_ONCE_REWRITE_TAC[SPLITP_LENGTH] >> fs[])
+       >> drule EVERY_MONOTONIC >> pop_assum kall_tac >> disch_then match_mp_tac >> rw[])
+  >> `!x. (λx. strlen x <= STRLEN t) x ==> (λx. strlen x <= SUC (STRLEN t)) x` by fs[]
+  >> drule EVERY_MONOTONIC >> pop_assum kall_tac >> disch_then match_mp_tac >> rw[]);
+
+val tokens_sum_less_eq = Q.prove(`!s f. SUM(MAP strlen (tokens f s)) <= strlen s`,
+  Induct >> Ho_Rewrite.PURE_ONCE_REWRITE_TAC[SWAP_FORALL_THM]
+  >> PURE_REWRITE_TAC[TOKENS_eq_tokens_sym,explode_thm,MAP_MAP_o]
+  >> recInduct TOKENS_ind >> rpt strip_tac
+  >> fs[TOKENS_def] >> pairarg_tac >> fs[] >> Cases_on `l` >> rw[] >> rfs[]
+  >> fs[SPLITP_NIL_FST] >> fs[SPLITP] >> every_case_tac
+  >> PURE_ONCE_REWRITE_TAC[SPLITP_LENGTH] >> fs[strlen_def,implode_def]);
+
+val tokens_not_nil = Q.prove(`!s f. EVERY (\x. x <> strlit "") (tokens f s)`,
+  Induct >> Ho_Rewrite.PURE_ONCE_REWRITE_TAC[SWAP_FORALL_THM]
+  >> PURE_REWRITE_TAC[TOKENS_eq_tokens_sym,explode_thm]
+  >> recInduct TOKENS_ind >> rpt strip_tac
+  >> rw[TOKENS_def] >> pairarg_tac >> fs[] >> reverse(Cases_on `l`)
+  >> fs[implode_def]);
+  
+val tokens_two_less = Q.prove(`!s f s1 s2. tokens f s = [s1;s2] ==> strlen s1 < strlen s /\ strlen s2 < strlen s`,
+  ntac 2 strip_tac >> qspecl_then [`s`,`f`] assume_tac tokens_sum_less_eq
+  >> qspecl_then [`s`,`f`] assume_tac tokens_not_nil
+  >> Induct >> Cases >> Induct >> Cases >> rpt strip_tac >> fs[]);
+
+val hexDigit_IMP_digit = Q.store_thm("hexDigit_IMP_digit",`!c. isDigit c ==> isHexDigit c`,
+  rw[isHexDigit_def,isDigit_def]);
+
+
+val parse_patch_header_side = Q.prove(`!s. parse_patch_header_side s = T`,
+  rw[fetch "-" "parse_patch_header_side_def",
+     fetch "-" "num_from_string_side_def",
+     fetch "-" "fromstring_side_def"]
+  >> TRY(match_mp_tac(MATCH_MP EVERY_MONOTONIC hexDigit_IMP_digit) >> fs[string_is_num_def])
+  >> TRY(match_mp_tac hexDigit_IMP_digit >> fs[string_is_num_def])
+  >> metis_tac[tokens_two_less]) |> update_precondition;
+
+val _ = translate patch_alg_def;
+
+val inputLines = process_topdecs`
+  fun inputLines fd =
+    let
+      fun loop() =
+        case inputLine fd of
+             NONE => []
+           | SOME l => l::loop()
+    in
+      loop()
+    end`
+
+val _ = append_prog inputLines;
+
+val _ = export_theory ();
